add some lemmans

zhi/problme1.v
@@ -17,13 +17,15 @@ Print leb.
 
 
 Definition Index := nat.
-(* for each element, we also record its original index, which is used to track
-   whether one elemnt is preceding another;
+(* for each element, we also record its index, which is its original position in
+   input array, and it will be used to track whether one elemnt is preceding another;
 *)
 Definition Stack := list (Index * nat).
 Definition Stacks := list Stack.
 Definition EmptyStacks: Stacks := nil.
 
+Definition Index_Of (e: Index * nat) := (fst e).
+Definition Value_Of (e: Index * nat) := (snd e).
 
 (**********************************
 
@@ -67,25 +69,95 @@ Require Import Coq.Init.Datatypes.
 Definition default: Stack := nil.
 
 Section Auxiliary.
+  (* to make sure that the cards are in order according to their index *)  
+  (*
+  Fixpoint Index_Increasing (cards: list (Index * nat)) : Prop :=
+    match cards with
+    | nil => True
+    | ((i, n) :: cards') =>
+        match cards' with
+        | nil => True
+        | ((i', n') :: cards'') =>
+          if leb i' i then
+            False
+          else
+            Index_Increasing cards' 
 
+        end
+    end.
+  *)
+
+  Inductive Index_Increasing_True: list (Index * nat) -> Prop :=
+    | Index_Inc1:
+        Index_Increasing_True nil 
+    | Index_Inc2: forall i n,
+        Index_Increasing_True ((i, n) :: nil) 
+    | Index_Inc3: forall i i' n' ls n,
+        i < i' ->
+        Index_Increasing_True ((i', n') :: ls) ->
+        Index_Increasing_True ((i, n) :: (i', n') :: ls).
+  
+  (* Stack_Indexes_Lt stack i: means all indexes of values in stack are less
+     than i; 
+  *)
+  Inductive Stack_Indexes_Lt: Stack -> nat -> Prop :=
+    | S_Less_Than1: forall i' i stack n n',
+        i' < i ->
+        Stack_Indexes_Lt stack n ->
+        Stack_Indexes_Lt ((i', n') :: stack) i
+    | S_Less_Than2: forall i,
+        Stack_Indexes_Lt nil i.
+
+  (* Stacks_Indexes_Lt stack i: means all indexes of values in stacks are less
+     than i; 
+  *)
+  Inductive Stacks_Indexes_Lt: Stacks -> nat -> Prop :=
+    | Less_Than1: forall stack i stacks,
+        Stack_Indexes_Lt stack i ->
+        Stacks_Indexes_Lt stacks i ->
+        Stacks_Indexes_Lt (stack :: stacks) i
+    | Less_Than2: forall i,
+        Stacks_Indexes_Lt nil i.
+
+  Lemma Stacks_Indexes_Lt_Subset: forall stack stacks i,
+    Stacks_Indexes_Lt (stack :: stacks) i ->
+    Stack_Indexes_Lt stack i /\ Stacks_Indexes_Lt stacks i.
+  Proof.
+    intros.
+    inversion H; subst; smack.
+  Qed.  
+  
   (* Precede stack stack': for each element in stack', there is an element
      in stack that precedes it; 
    *)
   Inductive Precede: Stack -> Stack -> Prop :=
     | Precede_NonEmpty: forall stack i' n' stack',
-        (exists i n, In (i, n) stack -> i <= i' /\ n <= n') ->
+        (exists i n, In (i, n) stack /\ i <= i' /\ n <= n') ->
         Precede stack stack' ->
         Precede stack ((i', n') :: stack')
     | Precede_Empty: forall stack,
         Precede stack nil.
 
+
+  Lemma In_Supperset(A: Type): forall (a a': A) (ls: list A),
+    In a ls ->
+      In a (a' :: ls).
+  Proof.
+    smack.
+  Qed.
   
   Lemma Add_Reserved: forall stack stack' a,
     Precede stack stack' ->
       Precede (a :: stack) stack'.
   Proof.    
-    (* ########### To Be Proved, which looks obvious *)
-    admit. 
+    intros. revert a.
+    induction H; smack.
+    constructor.
+    exists x, x0.
+    specialize (In_Supperset (Index * nat) (x, x0) (a0, b) stack H1).
+    smack.
+    apply IHPrecede.
+    constructor.
   Qed.
 
 
@@ -111,6 +183,7 @@ Section Auxiliary.
   *)
   Lemma Precede_Reserved: forall a stacks stacks' i,
     Insert_Rule a stacks stacks' ->
+    Stacks_Indexes_Lt stacks (Index_Of a) ->
     (forall j, j >= 1 -> j <= ((length stacks) - 1) -> 
                Precede (nth (j-1) stacks default) (nth j stacks default)) ->  
     i >= 1 ->
@@ -131,21 +204,58 @@ Section Auxiliary.
     destruct i; smack.
     destruct i; smack.
 *)
+(*
+    intros a stacks stacks' i H. revert i.
+    induction H.
+  - smack.
+    specialize (H1 i0 H2 H3).
+    destruct i0; smack.
+    destruct i0; smack.
+    apply Add_Reserved; auto.
+  - intros.
+    specialize (Insert_Rule_Property (i, n) stacks stacks' H1).
+    intros.
+    destruct H5. 
+    assert (HA1: length (stack :: stacks') = (length stacks') + 1).
+    apply Length_Inc1.
+    rewrite -> HA1 in *.
+    rewrite H5 in *.
+    
+    specialize (H2 i0 H3 H4).
+    destruct i0; smack.
+    destruct i0; smack.    
+*)    
+
     intros a stacks stacks' i H. revert i.
     induction H; smack.
-  - specialize (H1 i0 H2 H3).
+  - specialize (H2 i0 H3 H4).
     destruct i0; smack.
     destruct i0; smack.
     apply Add_Reserved; auto.
   - specialize (Insert_Rule_Property (i, n) stacks stacks' H1).
     smack.
-    rewrite H5 in *.
-    specialize (H2 i0 H3 H4).
+    rewrite H6 in *.    
+    specialize (H3 i0 H4 H5).
     destruct i0; smack.
-    destruct i0; smack.    
-    
-    
-    
+    destruct i0; smack.
+    + admit. (* ######### *)
+      
+
+
+      
+    + remember (S i0) as v.
+      assert(i0 = v -1) as HA1. omega.
+      rewrite HA1 in *.      
+      apply IHInsert_Rule; smack.
+      destruct v; smack.
+      remember (S v) as k.
+      assert(v - 0 = k - 1) as HA1. omega.
+      rewrite HA1 in H2.
+      assert (k >= 1 /\ k <= length stacks - 1). omega.
+      inversion H8.
+      admit.
+    + admit.
+      
   Qed.
 
  
@@ -156,10 +266,10 @@ End Auxiliary.
 Lemma lemma1: forall cards InitialStacks ResultStacks i,
   PatienceSolitaire_Rule cards InitialStacks ResultStacks ->
   (* requirement for the initial stack *)
-  (forall j, j >= 2 -> j <= length InitialStacks -> 
+  (forall j, j >= 1 -> j <= ((length InitialStacks) - 1) -> 
              Precede (nth (j-1) InitialStacks default) (nth j InitialStacks default)) ->
-  i >= 2 -> 
-  i <= length ResultStacks ->
+  i >= 1 -> 
+  i <= (length ResultStacks - 1) ->
   Precede (nth (i-1) ResultStacks default) (nth i ResultStacks default).
 Proof.
   induction cards.
